![[../../assets/image 28.png|image 28.png]]

## 傅里叶变换

$$X[0] = 2e^{0} + 1e^{0} + 3e^{0} + 0e^{0} = 2 + 1 + 3 + 0 = 6$$

$$X[1] = 2e^{0} + 1e^{-j\frac{\pi}{2}} + 3e^{-j\pi} + 0e^{-j\frac{3\pi}{2}}= 2 + 1(-j) + 3(-1) + 0 = 2 - j - 3 = -1 - j$$

$$X[2] = 2e^{0} + 1e^{-j\pi} + 3e^{-j2\pi} + 0e^{-j3\pi}= 2 + 1(-1) + 3(1) + 0 = 2 - 1 + 3 = 4$$

$$X[3] = 2e^{0} + 1e^{-j\frac{3\pi}{2}} + 3e^{-j3\pi} + 0e^{-j\frac{9\pi}{2}}= 2 + 1(j) + 3(-1) + 0 = 2 + j - 3 = -1 + j$$

离散傅里叶变换结果为: $X[k] = [6, -1-j, 4, -1+j]$

## 逆变换

$$x[0] = \frac{1}{4}[6e^{0} + (-1-j)e^{0} + 4e^{0} + (-1+j)e^{0}]= \frac{1}{4}[6 + (-1-j) + 4 + (-1+j)] = \frac{1}{4}[8] = 2$$

$$x[1] = \frac{1}{4}[6e^{0} + (-1-j)e^{j\frac{\pi}{2}} + 4e^{j\pi} + (-1+j)e^{j\frac{3\pi}{2}}]= \frac{1}{4}[6 + (-1-j)(j) + 4(-1) + (-1+j)(-j)] = 1$$

$$x[2] = \frac{1}{4}[6e^{0} + (-1-j)e^{j\pi} + 4e^{j2\pi} + (-1+j)e^{j3\pi}]= \frac{1}{4}[6 + (-1-j)(-1) + 4(1) + (-1+j)(-1)]=3$$

$$x[3] = \frac{1}{4}[6e^{0} + (-1-j)e^{j\frac{3\pi}{2}} + 4e^{j3\pi} + (-1+j)e^{j\frac{9\pi}{2}}]= \frac{1}{4}[6 + (-1-j)(-j) + 4(-1) + (-1+j)(j)] = 0$$

逆变换结果为:

$$x[n] = [2, 1, 3, 0]$$